examples/map/MapHeader.v
@@ -29,28 +29,17 @@ Section RESOURCE.
   Definition map_points_to (k: Z) (v: Z): iProp :=
     OwnM (map_points_to_r k v).
 
-  (* Definition S_map_points_to {n} (k: Z) (v: Z): SRFSyn.t n :=
-    (<ownm> (map_points_to_r k v))%SRF. *)
-
   Definition pending_r: pendingRA :=
     (Excl.just tt, ε).
 
   Definition pending: iProp :=
     OwnM pending_r.
     
-  (* Definition S_pending {n}: SRFSyn.t n :=
-    (<ownm> pending_r)%SRF. *)
-
-
-  (* Definition pending `{@GRA.inG MapRA0 Σ} `{@GRA.inG MapRA Σ}: iProp :=
-      pending0 ∗ pending1. *)
-
   Fixpoint initial_points_tos (sz: nat): iProp :=
     match sz with
     | 0 => True%I
     | S sz' => initial_points_tos sz' ∗ map_points_to sz' 0
     end.
-
 
   Definition initial_r: (Z ==> (Excl.t Z))%ra := (fun _ => Excl.just 0%Z).
   
@@ -75,12 +64,6 @@ Section RESOURCE.
   Definition unallocated (sz: Z): iProp :=
     OwnM (unallocated_r sz).
 
-
-
-
-  (* Definition MapRA0: URA.t := URA.prod (Excl.t unit) (Excl.t Z).
-  Context `{@GRA.inG MapRA0 Γ}. *)
-
   Definition pending0RA: URA.t := Excl.t unit.
   Context `{@GRA.inG pending0RA Γ}. 
 
@@ -89,118 +72,21 @@ Section RESOURCE.
   Definition pending0: iProp :=
     OwnM pending0_r.
 
-  (* Definition CallableRA : URA.t := Excl.t unit.
-  Context `{@GRA.inG CallableRA Γ}.
-  Definition callable_r :(@URA.car CallableRA) := Some tt.
-
-  Definition callable : iProp := OwnM callable_r.
-
-  Definition MapStateRA : URA.t := Auth.t (Excl.t (((Z->Z) * Z) * val)).
-  Context `{@GRA.inG MapStateRA Γ}.
-  Definition mapstate_r st : MapStateRA := Auth.white ((Excl.just st) : @URA.car (Excl.t (((Z->Z) * Z) * val))%ra).
-  Definition mapstate st : iProp := OwnM (mapstate_r st).
-
-  Definition mapstate_auth_r st : MapStateRA := Auth.black ((Excl.just st) : @URA.car (Excl.t (((Z->Z) * Z) * val))%ra).
-  Definition mapstate_auth st : iProp := OwnM (mapstate_auth_r st).
-
-  Definition mapstate_full st : iProp := mapstate_auth st ∗ mapstate st.
-
-  Lemma mapstate_update st st0 : mapstate_full st -∗ #=> mapstate_full st0.
-  Proof. 
-    iIntros "[H0 H1]". unfold mapstate_full, mapstate, mapstate_auth, mapstate_auth_r, mapstate_r.
-    iCombine "H0 H1" as "H".  
-    iPoseProof (OwnM_Upd with "H") as "H".
-    { 
-      instantiate (1:= (Auth.black ((Excl.just st0): @URA.car (Excl.t (((Z->Z) * Z) * val))) ⋅ Auth.white ((Excl.just st0): @URA.car (Excl.t (((Z->Z) * Z) * val))))).
-      ii. ur in H3. des_ifs. des. rewrite URA.unit_idl in H3.
-      unfold URA.extends in H3. des. ur in H3. ur.
-      rewrite URA.unit_idl. split.
-      { exists ctx. ur. des_ifs. }
-      des_ifs. ur. ss.
-    } 
-    iMod "H". iModIntro. 
-    iDestruct "H" as "[H0 H1]". iFrame.
-  Qed.
-
-  Lemma mapstate_auth_unique st st0: mapstate_auth st -∗ mapstate_auth st0 -∗ False.
-  Proof.
-    iIntros "H0 H1". iCombine "H0 H1" as "H".
-    iOwnWf "H". ur in H3. eauto.
-  Qed.
-
-  Lemma mapstate_upd st st0: mapstate_auth st -∗ mapstate st0 -∗ #=> mapstate_full st. 
-  Proof.
-    iIntros "H0 H1". 
-    unfold mapstate_full, mapstate, mapstate_auth, mapstate_auth_r, mapstate_r.
-    iCombine "H0 H1" as "H".
-    iPoseProof (OwnM_Upd with "H") as "H".
-    { 
-      instantiate (1:= (Auth.black ((Excl.just st): @URA.car (Excl.t (((Z->Z) * Z) * val))) ⋅ Auth.white ((Excl.just st): @URA.car (Excl.t (((Z->Z) * Z) * val))))).
-      ii. ur in H3. des_ifs. des. rewrite URA.unit_idl in H3.
-      unfold URA.extends in H3. des. ur in H3. ur.
-      rewrite URA.unit_idl. split.
-      { exists ctx. ur. des_ifs. }
-      des_ifs.
-    } 
-    iMod "H". iModIntro. 
-    iDestruct "H" as "[H0 H1]". iFrame.
-  Qed.
-
-  Lemma mapstate_eq st st0: mapstate_auth st -∗ mapstate st0 -∗ ⌜st = st0⌝.
-  Proof.
-    iIntros "H0 H1".
-    unfold mapstate_full, mapstate, mapstate_auth, mapstate_auth_r, mapstate_r.
-    iOwnWf "H0". eapply Auth.black_wf in H3.
-    iCombine "H0 H1" as "H".
-    iOwnWf "H". eapply Auth.auth_included in H4. des.
-    iPureIntro.
-    eapply (Excl.extends H3) in H4. 
-    des. clarify. 
-  Qed. *)
-  
-  (* Definition initialized0_r ofs: MapRA0 := (ε, Excl.just ofs).
-
-  Definition initialized0 ofs: iProp :=
-    OwnM (initialized0_r ofs).
-    
-  Fixpoint initial0 (sz: nat): iProp :=
-    match sz with
-    | 0 => True%I
-    | S sz' => initial0 sz' ∗ initialized0 sz'
-    end. *)
-
   Global Opaque map_points_to pending pending0 initial_map black_map unallocated.
 
 End RESOURCE.
-
 
 Module MapRA.
   Class t
     `{_W: CtxWD.t}
     `{@GRA.inG pendingRA Γ}
     `{@GRA.inG pending0RA Γ}
-    (* `{@GRA.inG CallableRA Γ} *)
-    (* `{@GRA.inG MapStateRA Γ} *)
     := MapRA: unit.
 
 End MapRA.
 
-Module MapRA0.
-  
-  Class t
-    `{_W: CtxWD.t}
-    `{@GRA.inG pending0RA Γ}
-    (* `{@GRA.inG CallableRA Γ} *)
-    (* `{@GRA.inG MapStateRA Γ} *)
-    := MapRA0: unit.
-
-End MapRA0.
-
 Section SPECS.
   Context `{_M: MapRA.t}.
-  (* Context `{@GRA.inG MapRA Γ}.
-  Context `{@GRA.inG MapRA0 Γ}.
-  Context `{@GRA.inG CallableRA Γ}. *)
 
   Definition init_spec: fspec :=
     mk_fspec_inv 0
@@ -209,8 +95,6 @@ Section SPECS.
                       (fun varg => ( ⌜varg = ([Vint sz]: list val)↑⌝
                                      ∗ ⌜(8 * (Z.of_nat sz) < modulus_64%Z)%Z⌝
                                      ∗ pending)%I),
-                                     (* exists N, inv u n N S_pending *)
-                                     (* inv u n PENDING S_pending *)
                       (fun vret => (⌜vret = Vundef↑⌝ ∗ initial_points_tos sz)%I)))).
 
   Definition init_specM: fspec :=
@@ -249,7 +133,7 @@ Section SPECS.
     mk_fspec_inv 0
     (fun _ _ => mk_simple (fun '(k, v) =>
                   (ord_top,
-                    (fun varg => (⌜varg = ([Vint k; Vint v])↑⌝ )%I),
+                    (fun varg => (⌜varg = ([Vint k; Vint v])↑⌝)%I),
                     (fun vret => True%I)))).  
 
   Definition set_by_user_spec: fspec :=
@@ -266,9 +150,9 @@ Section SPECS.
                   (ord_top,
                     (fun varg => (⌜varg = ([Vint k])↑⌝)%I),
                     (fun vret => True%I)))).  
+
+  Definition Map0_initial_cond : iProp := True%I.
   
-  (* Definition Map0_initial_cond : iProp := mapstate_full ((fun (_: Z) => 0%Z, 0%Z), Vnullptr). *)
-  Definition Map0_initial_cond : iProp := emp.
   Definition Map_initial_cond : iProp := initial_map ∗ pending0 ∗ Map0_initial_cond.
 
   Definition MapStb: alist gname fspec :=
@@ -278,12 +162,6 @@ Section SPECS.
     Seal.sealing "stb" [("init", init_specM); ("get", get_specM); ("set", set_specM); ("set_by_user", set_by_user_specM)].
 End SPECS.
 Global Hint Unfold MapStb MapStbM: stb.
-
-
-
-Definition set `{Dec K} V (k: K) (v: V) (f: K -> V): K -> V := fun k0 => if dec k k0 then v else f k0.
-
-
 
 Section PROOF.
   Context `{Σ: GRA.t}.
@@ -325,17 +203,18 @@ Section PROOF.
   Qed.
 End PROOF.
 
-
 Notation pget := (p0 <- trigger sGet;; p0 <- p0↓ǃ;; Ret p0) (only parsing).
 Notation pput p0 := (trigger (sPut p0↑)) (only parsing).
 
-Fixpoint set_nth A (n:nat) (l:list A) (new:A) {struct l} : option (list A) :=
-  match n, l with
-  | O, x :: l' => Some (new :: l')
-  | O, other => None
-  | S m, [] => None
-  | S m, x :: t => option_map (cons x) (set_nth m t new)
-  end.
+(* Definition set `{Dec K} V (k: K) (v: V) (f: K -> V): K -> V := fun k0 => if dec k k0 then v else f k0. *)
+
+(* Fixpoint set_nth A (n:nat) (l:list A) (new:A) {struct l} : option (list A) := *)
+(*   match n, l with *)
+(*   | O, x :: l' => Some (new :: l') *)
+(*   | O, other => None *)
+(*   | S m, [] => None *)
+(*   | S m, x :: t => option_map (cons x) (set_nth m t new) *)
+(*   end. *)
 
 
 (* 
