examples/map/MapIMproof.v
@@ -1,4 +1,4 @@
-Require Import MapHeader MapI MapM HoareDef SimModSem SimModSemFacts.
+Require Import MapHeader MapI MapM HoareDef SimModSem.
 Require Import Coqlib.
 Require Import ImpPrelude.
 Require Import Skeleton.
@@ -19,7 +19,7 @@ Require Import HTactics ProofMode IPM.
 Require Import OpenDef.
 Require Import Mem1 MemOpen STB Invariant.
 
-Require Import SimModSemFacts IProofMode IRed ITactics.
+Require Import IProofMode IRed ITactics.
 
 
 Require Import sProp sWorld World SRF.
@@ -29,225 +29,301 @@ Set Implicit Arguments.
 
 Local Open Scope nat_scope.
 
-
-
-
 Section SIMMODSEM.
-  Context `{_M: MapRA0.t}.
-
-  (* Context `{_W: CtxWD.t}.
-  Context `{@GRA.inG pending0RA Γ}.
-  Context `{@GRA.inG CallableRA Γ}.
-  Context `{@GRA.inG MapStateRA Γ}. *)
-
+  Context `{_M: MapRA.t}.
   Context `{@GRA.inG memRA Γ}. 
         
   Variable GlobalStbM: Sk.t -> gname -> option fspec.
   Hypothesis STBINCLM: forall sk, stb_incl (to_stb MemStb) (GlobalStbM sk).
-  (* Hypothesis STB_getM: forall sk, (GlobalStbM sk) "get" = Some get_specM. *)
   Hypothesis STB_setM: forall sk, (GlobalStbM sk) "set" = Some set_specM.
 
-  Section LEMMA. 
+  Lemma pending0_unique:
+    pending0 -∗ pending0 -∗ False%I.
+  Proof.
+    Local Transparent pending0.
+    iIntros "H0 H1". iCombine "H0 H1" as "H".
+    iOwnWf "H" as WF. exfalso.
+    rr in WF. ur in WF. unseal "ra". des. ur in WF. ss.
+  Qed.
+  
+  Definition fun_to_list (f: Z -> Z) (sz: nat) : list val :=
+    map (fun i:nat => Vint (f i)) (seq 0 sz).
 
-    (* Lemma callable_unique:
-      callable -∗ callable -∗ False%I.
-    Proof.
-      Local Transparent callable.
-      iIntros "H0 H1". iCombine "H0 H1" as "H".
-      iOwnWf "H". exfalso. clear -H3.
-      rr in H3. ur in H3. unseal "ra". des. ur in H3. ss.
-    Qed.     *)
+  Definition Ist: Any.t -> Any.t -> iProp :=
+    fun st_src st_tgt =>
+       ((⌜st_src = (fun (_: Z) => 0%Z, 0%Z)↑ /\ st_tgt = Vnullptr↑⌝)
+        ∨
+        (pending0 ∗ ∃ blk ofs (f: Z -> Z) (sz: Z), 
+            ⌜st_src = (f, sz)↑ /\  st_tgt = (Vptr blk ofs)↑⌝ 
+            ∗ [∗ list] i↦v ∈ (fun_to_list f (Z.to_nat sz)), PointsTo (blk, (ofs + i))%Z v)
+       )%I.
 
-    Lemma pending0_unique:
-      pending0 -∗ pending0 -∗ False%I.
-    Proof.
-      Local Transparent pending0.
-      iIntros "H0 H1". iCombine "H0 H1" as "H".
-      iOwnWf "H". exfalso. clear - H1.
-      rr in H1. ur in H1. unseal "ra". des. ur in H1. ss.
-    Qed.
+  Lemma repeat_update {A} i n (v v' w: A):
+    <[i:=v]> (repeat v i ++ v' :: repeat w n) = repeat v (i+1) ++ repeat w n.
+  Proof.
+    replace i with (length (repeat v i) + 0) at 1; cycle 1.
+    { rewrite repeat_length. nia. }
+    rewrite ->insert_app_r, repeat_app, <-app_assoc. eauto.
+  Qed.
 
-    Lemma points_to_get_split blk ofs l k v
-          (GET: nth_error l k = Some v)
-      :
-      OwnM((blk, ofs) |-> l) -∗ (OwnM((blk, (ofs + k)%Z) |-> [v])) ** ((OwnM((blk, (ofs + k)%Z) |-> [v]) -* OwnM((blk, ofs) |-> l))).
-    Proof.
-      revert blk ofs k v GET. induction l; ss; i.
-      { destruct k; ss. }
-      destruct k; ss.
-      { clarify. iIntros "H". rewrite points_to_split.
-        iDestruct "H" as "[H0 H1]". iSplitL "H0".
-        { rewrite Z.add_0_r. ss. }
-        iIntros "H". iSplitL "H".
-        { rewrite Z.add_0_r. ss. }
-        { ss. }
-      }
-      { iIntros "H". rewrite points_to_split.
-        iDestruct "H" as "[H0 H1]".
-        iPoseProof (IHl with "H1") as "H1"; eauto.
-        iDestruct "H1" as "[H1 H2]".
-        replace (ofs + Z.pos (Pos.of_succ_nat k))%Z with (ofs + 1 + k)%Z by lia.
-        iSplitL "H1"; auto. iIntros "H1". iSplitL "H0"; auto.
-        iApply "H2". auto.
-      }
-    Qed.
+  Lemma repeat_fun_to_list (n: nat):
+    repeat (Vint 0) n = fun_to_list (λ _ : Z, 0%Z) n.
+  Proof.
+    unfold fun_to_list. induction n; eauto.
+    replace (S n) with (n+1) by nia.
+    rewrite ->repeat_app, seq_app, map_app, IHn. eauto.
+  Qed.
 
-    Lemma set_nth_success A (l: list A) (k: nat) v
-          (SZ: k < length l)
-      :
-      exists l', set_nth k l v = Some l'.
-    Proof.
-      revert k v SZ. induction l; ss; i.
-      { exfalso. lia. }
-      { destruct k; ss; eauto.
-        hexploit IHl; eauto.
-        { instantiate (1:=k). lia. }
-        i. des. rewrite H1. eauto.
-      }
-    Qed.
+  Lemma fun_to_list_lookup (f: Z -> Z) (sz: nat) (i: nat)
+    (LT: i < sz)
+    :
+    fun_to_list f sz !! i = Some (Vint (f i)).
+  Proof.
+    unfold fun_to_list.
+    rewrite ->list_lookup_fmap, lookup_seq_lt; try nia. eauto.
+  Qed.
 
-    Lemma points_to_set_split blk ofs l k v l'
-          (GET: set_nth k l v = Some l')
-      :
-      OwnM((blk, ofs) |-> l) -∗ (∃ v', OwnM((blk, (ofs + k)%Z) |-> [v'])) ** ((OwnM((blk, (ofs + k)%Z) |-> [v]) -* OwnM((blk, ofs) |-> l'))).
-    Proof.
-      revert blk ofs k v l' GET. induction l; ss; i.
-      { destruct k; ss. }
-      destruct k; ss.
-      { clarify. iIntros "H". rewrite points_to_split.
-        iDestruct "H" as "[H0 H1]". iSplitL "H0".
-        { rewrite Z.add_0_r. iExists _. ss. }
-        iIntros "H". iEval (rewrite points_to_split). iSplitL "H".
-        { rewrite Z.add_0_r. ss. }
-        { ss. }
-      }
-      { iIntros "H". rewrite points_to_split.
-        iDestruct "H" as "[H0 H1]".
-        unfold option_map in GET. des_ifs.
-        iPoseProof (IHl with "H1") as "H1"; eauto.
-        iDestruct "H1" as "[H1 H2]". iDestruct "H1" as (v') "H1".
-        replace (ofs + Z.pos (Pos.of_succ_nat k))%Z with (ofs + 1 + k)%Z by lia.
-        iSplitL "H1"; auto. iIntros "H1".
-        iEval (rewrite points_to_split). iSplitL "H0"; auto.
-        iApply "H2". auto.
-      }
-    Qed.
+  Lemma fun_to_list_update (f: Z -> Z) (sz: nat) (i: nat) (v: Z)
+    :
+    <[i := Vint v]> (fun_to_list f sz) = fun_to_list (<[Z.of_nat i := v]> f) sz.
+  Proof.
+    unfold fun_to_list. revert i. induction sz; i; eauto.
+    replace (S sz) with (sz + 1) by nia.
+    rewrite ->!seq_app, !map_app.
+    assert (CASE: i < sz \/ i >= sz) by nia.
+    des.
+    - rewrite insert_app_l; cycle 1.
+      { rewrite ->map_length, seq_length. nia. }
+      rewrite IHsz. s. do 3 f_equal.
+      rewrite fn_lookup_insert_ne; eauto. nia.
+    - assert (Iadd: length (map (λ i0 : nat, Vint (f i0)) (seq 0 sz)) + (i - sz) = i).
+      { rewrite ->map_length, seq_length. nia. }
+      s. rewrite -IHsz -{1 2}Iadd -{4}(app_nil_r (seq 0 sz)) map_app. 
+      rewrite ->!insert_app_r, <-app_assoc. f_equal. s.
+      assert (CASE': i = sz \/ i > sz) by nia.
+      des; subst.
+      + rewrite ->fn_lookup_insert, Nat.sub_diag. eauto.
+      + rewrite ->fn_lookup_insert_ne; try nia.
+        destruct (i-sz) eqn: EQ; try nia. eauto.
+  Qed.
+  
+  Let Mem := HMem (fun _ => false).
 
-    Lemma set_nth_map A B (f: A -> B) k l v
-      :
-      set_nth k (List.map f l) (f v) = option_map (List.map f) (set_nth k l v).
-    Proof.
-      revert k v. induction l; ss; i.
-      { destruct k; ss. }
-      { destruct k; ss. rewrite IHl. unfold option_map. des_ifs. }
-    Qed.
+  Lemma simF_init:
+    HModPair.sim_fun
+      (HMod.add (MapM.HMap GlobalStbM) Mem) (HMod.add MapI.Map Mem)
+      (IstProd Ist IstEq) "init".
+  Proof.
+    r. i. pattern (MapM.HMap GlobalStbM) at 1. rewrite MapM.HMap_unfold. s.
+    pattern MapI.Map at 1. rewrite MapI.Map_unfold. s. i. iIntros "IST".
 
-    Lemma nth_error_map A B (f: A -> B) k l
-      :
-      nth_error (List.map f l) k = option_map f (nth_error l k).
-    Proof.
-      revert k. induction l; ss; i.
-      { destruct k; ss. }
-      { destruct k; ss. }
-    Qed.
+    unfold cfunU, initF, MapI.initF, interp_sb_hp, HoareFun, ccallU. s.
+    st. iDestruct "ASM" as "(W & (%Y & %M & P0) & %X)". subst.
+    st. iDestruct "IST" as (? ? ? ?) "(%& [%|(P & _)] &%)"; des; subst; cycle 1.
+    { iExFalso. iApply (pending0_unique with "P P0"). }
+    inline_r.
+    st. force. instantiate (1:= x).
+    st. force. instantiate (1:= [Vint x]↑).
+    st. force. iSplitR; eauto.
+    (* todo: make the following as a lemma *)
+    st. rewrite interp_hAGEs_hapc. st. unfold HoareAPC. st. rewrite unfold_APC.
+    st. destruct y4; cycle 1.
+    { unfold guarantee, triggerNB. st. inv y6. }
+    
+    unfold ModSem.run_l. rewrite !Any.pair_split. fold ModSem.run_l.
+    
+    st. iDestruct "GRT" as "[GRT %]". iDestruct "GRT" as ( ? ) "(% & POINTS)". subst. st.
+    unfold ModSem.run_l. rewrite ! Any.pair_split. fold ModSem.run_l.
+    st. force. st. force. iSplitL "W". { iFrame. eauto. }
+    rewrite Any.upcast_downcast in G. inv G. inv G0. st.
 
-    Lemma repeat_nth A (a: A) n k
-          (RANGE: k < n)
-      :
-      nth_error (List.repeat a n) k = Some a.
-    Proof.
-      revert k RANGE. induction n; ss; i.
-      { lia. }
-      { destruct k; ss. rewrite IHn; eauto. lia. }
-    Qed.
+    iPoseProof (points_to_conv with "POINTS") as "POINTS".
+    replace (repeat Vundef x) with (repeat (Vint 0) (x-x) ++ repeat Vundef x); cycle 1.
+    { rewrite Nat.sub_diag. eauto. }
+    match goal with |- context[ITree.iter ?f 0%Z] =>
+      replace (ITree.iter f 0%Z) with (ITree.iter f (x-x)%Z) by (f_equal; nia)
+    end.
 
-    Lemma set_nth_length A k (a: A) l l'
-          (SET: set_nth k l a = Some l')
-      :
-      length l' = length l.
-    Proof.
-      revert l l' SET. induction k; ss; i.
-      { destruct l; ss. clarify. }
-      { destruct l; ss. unfold option_map in *. des_ifs.
-        ss. f_equal. eauto.
-      }
-    Qed.
+    iStopProof. cut (x <= x); [|lia].
+    generalize x at 1 4 5 11. intros n. induction n; i; iIntros "(PD & PTS)".
+    {
+      rewrite unfold_iter_eq. st. des_ifs. { exfalso. nia. }
+      st. iSplitL; [|eauto].
+      iExists _, _, _, _; iSplitR; eauto; iSplitL; eauto.
+      iRight. iFrame. iExists b, 0%Z, (fun _ => 0%Z), x.
+      iSplit; eauto.
+      rewrite ->app_nil_r, Nat.sub_0_r, repeat_fun_to_list, Nat2Z.id. eauto.
+    }
 
-    Lemma set_nth_error A k (a: A) l l' k'
-          (SET: set_nth k l a = Some l')
-      :
-      nth_error l' k' = if Nat.eq_dec k' k then Some a else nth_error l k'.
-    Proof.
-      revert a l l' k' SET. induction k; ss; i.
-      { destruct l; ss. clarify. des_ifs. destruct k'; ss. }
-      { destruct l; ss. unfold option_map in *. des_ifs; ss.
-        { erewrite IHk; eauto. des_ifs. }
-        { destruct k'; ss. erewrite IHk; eauto. des_ifs. }
-      }
-    Qed.
+    rewrite unfold_iter_eq. st. des_ifs; cycle 1. { exfalso. nia. }
+    st. unfold scale_int at 1. des_ifs; cycle 1.
+    { exfalso. eapply n0. eapply Z.divide_factor_r. }
+    st. inline_r.
+    st. force. instantiate (1:= (b, (x - S n)%Z, Vint 0)).
+    st. force. instantiate (1:= [Vptr b (x - (S n))%Z; Vint 0]↑).
+    st. force.
+    iPoseProof (big_sepL_insert_acc with "PTS") as "(PT & CTN)".
+    { instantiate (2:= (x - (S n))).
+      rewrite lookup_app_r; rewrite repeat_length; try nia.
+      rewrite Nat.sub_diag. eauto.
+    }
 
-    Lemma repeat_map A B (f: A -> B) (a: A) n
-      :
-      map f (repeat a n) = repeat (f a) n.
-    Proof.
-      induction n; ss. f_equal; auto.
-    Qed.
+    rewrite ->!Z.add_0_l, Zpos_P_of_succ_nat, <-Nat2Z.inj_succ, Nat2Z.inj_sub; try nia.
+    iSplitL "PT".
+    { iSplitL; cycle 1.
+      { iPureIntro. do 3 f_equal. rewrite Z.div_mul; nia. }
+      iExists Vundef. iFrame.
+      iPureIntro. do 3 f_equal. rewrite Z.div_mul; nia.
+    }
+    (* todo: make the following as a lemma *)
+    st. rewrite interp_hAGEs_hapc. st. unfold HoareAPC. st. rewrite unfold_APC.
+    st. destruct y3; cycle 1.
+    { unfold guarantee, triggerNB. st. inv y5. }
 
-    Lemma unfold_iter (E : Type -> Type) (A B : Type) (f : A -> itree E (A + B)) (x : A)
-      :
-      ITree.iter f x = lr <- f x;;
-                       match lr with
-                       | inl l => tau;; ITree.iter f l
-                       | inr r => Ret r
-                       end.
-    Proof.
-      eapply bisim_is_eq. eapply unfold_iter.
-    Qed.
+    st. iDestruct "GRT" as "[[GRT %] %]". subst.
+    st. iPoseProof ("CTN" with "GRT") as "PTS".
+    rewrite ->!Zpos_P_of_succ_nat, <-!Nat2Z.inj_succ.
+    replace (x - S n + 1)%Z with (x - n)%Z by nia.
+    iApply IHn; try nia. iFrame.
+    rewrite repeat_update.
+    eapply eq_ind. { iApply "PTS". }
+    do 3 f_equal. nia.
+  Qed.
 
-    Lemma points_to_nil blk ofs
-      :
-      ((blk, ofs) |-> []) = ε.
-    Proof.
-      Local Transparent URA.unit.
-      ss. unfold points_to, Auth.white. f_equal.
-      rewrite unfold_points_to.
-      extensionality _blk. extensionality _ofs. unfold andb. des_ifs.
-      exfalso. ss. lia.
-    Qed.
+  Lemma simF_get:
+    HModPair.sim_fun
+      (HMod.add (MapM.HMap GlobalStbM) Mem) (HMod.add MapI.Map Mem)
+      (IstProd Ist IstEq) "get".
+  Proof.
+    r. i. pattern (MapM.HMap GlobalStbM) at 1. rewrite MapM.HMap_unfold. s.
+    pattern MapI.Map at 1. rewrite MapI.Map_unfold. s. i. iIntros "IST".
 
-    Lemma points_to_app blk ofs l0 l1
-      :
-      (blk, ofs) |-> (l0 ++ l1) = ((blk, ofs) |-> l0) ⋅ ((blk, (ofs + strings.length l0)%Z) |-> l1).
-    Proof.
-      revert ofs l1. induction l0; i; ss.
-      { rewrite points_to_nil. rewrite URA.unit_idl. ss.
-        replace (ofs + 0)%Z with ofs; ss. lia.
-      }
-      { rewrite points_to_split. rewrite (points_to_split blk ofs a l0).
-        erewrite IHl0. rewrite URA.add_assoc. f_equal; ss.
-        replace (ofs + Z.pos (Pos.of_succ_nat (strings.length l0)))%Z with
-          (ofs + 1 + strings.length l0)%Z; ss. lia.
-      }
-    Qed.
+    unfold cfunU, getF, MapI.getF, interp_sb_hp, HoareFun, ccallU. s.
+    st. iDestruct "ASM" as "(W & % & %)". subst. st.
+    rewrite Any.upcast_downcast in G. inv G. inv G0.
+    iDestruct "IST" as (? ? ? ?) "(%& [%|(P & IST)] &%)";
+      [|iDestruct "IST" as (? ? ? ?) "(% & M)"];
+      des; subst; unfold ModSem.run_l, assume; rewrite ! Any.pair_split.
+    { st. nia. }
+    st. force. instantiate (1:= (Vint (f y3))↑).
+    unfold scale_int. des_ifs; cycle 1.
+    { exfalso. eapply n. eapply Z.divide_factor_r. }
+    st. force. iSplitL "W". { eauto. }
 
-    Lemma OwnM_combine M `{@GRA.inG M Γ} a0 a1
-      :
-      (OwnM a0 ** OwnM a1) -∗ OwnM (a0 ⋅ a1).
-    Proof.
-      iIntros "[H0 H1]". iCombine "H0 H1" as "H". auto.
-    Qed.
+    rewrite Z_div_mult; try nia.
+    iPoseProof (big_sepL_lookup_acc with "M") as "(IP & M)".
+    { apply fun_to_list_lookup with (i:=Z.to_nat y3). nia. }
+    inline_r.
+    st. force. instantiate (1:= (blk, (ofs + y3)%Z, Vint (f y3))).
+    st. force.
+    st. force. rewrite Z2Nat.id; try nia.
+    iSplitL "IP"; eauto.
+    (* todo: make the following as a lemma *)
+    st. rewrite interp_hAGEs_hapc. st. unfold HoareAPC. st. rewrite unfold_APC.
+    st. destruct y4; cycle 1.
+    { unfold guarantee, triggerNB. st. inv y6. }
+    
+    st. iDestruct "GRT" as "[[GRT %] %]". subst.
+    st. iSplitL; eauto.
+    iExists _, _, _, _; iSplitR; eauto; iSplitL; eauto.
+    iRight. iFrame. iExists blk, ofs, f, sz.
+    iPoseProof ("M" with "GRT") as "M". iFrame. eauto.
+  Qed.
 
-  End LEMMA.
+  Lemma simF_set:
+    HModPair.sim_fun
+      (HMod.add (MapM.HMap GlobalStbM) Mem) (HMod.add MapI.Map Mem)
+      (IstProd Ist IstEq) "set".
+  Proof.
+    r. i. pattern (MapM.HMap GlobalStbM) at 1. rewrite MapM.HMap_unfold. s.
+    pattern MapI.Map at 1. rewrite MapI.Map_unfold. s. i. iIntros "IST".
+    
+    unfold cfunU, setF, MapI.setF, interp_sb_hp, HoareFun, ccallU. s.
+    st. iDestruct "ASM" as "(W & % & %)". subst. st.
+    rewrite Any.upcast_downcast in G. inv G. inv G0.
+    iDestruct "IST" as (? ? ? ?) "(%& [%|(P & IST)] &%)";      
+      [|iDestruct "IST" as (? ? ? ?) "(% & M)"];
+      des; subst; unfold ModSem.run_l, assume; rewrite ! Any.pair_split.
+    { st. nia. }
+    st. force. instantiate (1:= Vundef↑).
+    rewrite ! Any.pair_split.
+    unfold scale_int. des_ifs; cycle 1.
+    { exfalso. eapply n. eapply Z.divide_factor_r. }
+    st. force. iSplitL "W". { eauto. }
 
-  (***** Move and rename: APC & HoareCall LEMMAS *****)
+    rewrite Z_div_mult; try nia.
+    iPoseProof (big_sepL_insert_acc with "M") as "(IP & M)".
+    { apply fun_to_list_lookup with (i:=Z.to_nat y4). nia. }
+    inline_r.
+    st. force. instantiate (1:= (blk, (ofs + y4)%Z, Vint y5)).
+    st. force.
+    st. force. rewrite Z2Nat.id; try nia.
+    iSplitL "IP"; eauto.
+    (* todo: make the following as a lemma *)
+    st. rewrite interp_hAGEs_hapc. st. unfold HoareAPC. st. rewrite unfold_APC.
+    st. destruct y3; cycle 1.
+    { unfold guarantee, triggerNB. st. inv y7. }
+    st. iDestruct "GRT" as "[[GRT %] %]". subst.
+    st. iSplitL; eauto.
 
+    iExists _, _, _, _; iSplitR; eauto; iSplitL; eauto.      
+    iRight. iFrame. iExists blk, ofs, (<[y4:=y5]> f), sz.
+    iPoseProof ("M" with "GRT") as "M".
+    rewrite ->fun_to_list_update, Z2Nat.id; try nia.
+    eauto.
+  Qed.
+
+  Lemma simF_set_by_user:
+    HModPair.sim_fun
+      (HMod.add (MapM.HMap GlobalStbM) Mem) (HMod.add MapI.Map Mem)
+      (IstProd Ist IstEq) "set_by_user".
+  Proof.
+    r. i. pattern (MapM.HMap GlobalStbM) at 1. rewrite MapM.HMap_unfold. s.
+    pattern MapI.Map at 1. rewrite MapI.Map_unfold. s. i. iIntros "IST".
+
+    unfold cfunU, set_by_userF, MapI.set_by_userF, interp_sb_hp, HoareFun, ccallU. s.
+    st. iDestruct "ASM" as "(W & % & %)". subst.
+    rewrite Any.upcast_downcast in G. inv G. inv G0.
+    st. rewrite STB_setM. st. unfold HoareCall.
+    force. instantiate (1:= mk_meta y0 y1 (y3, y)).
+    force. instantiate (1:= [Vint y3; Vint y]↑).
+    st. force. iSplitL "W". { iFrame. eauto. }
+    call; [eauto|].
+    st. iDestruct "ASM" as "(W & _ & %)". subst.
+    force. st. force. iSplitL "W". { eauto. } 
+    rewrite G0. st. eauto.
+  Qed.
+  
+  Theorem sim: HModPair.sim (HMod.add (MapM.HMap GlobalStbM) Mem) (HMod.add MapI.Map Mem) (IstProd Ist IstEq).
+  Proof.
+    sim_init.
+    - iIntros "[H0 H1]". iFrame.
+      iExists _, _, _, _; iSplitR; eauto; iSplitL; eauto.
+      iLeft; eauto.
+    - iApply simF_init. eauto.
+    - iApply simF_get. eauto.
+    - iApply simF_set. eauto.
+    - iApply simF_set_by_user. eauto.
+    - iApply isim_reflR. eauto.
+    - iApply isim_reflR. eauto.
+    - iApply isim_reflR. eauto.
+    - iApply isim_reflR. eauto.
+    - iApply isim_reflR. eauto.
+  Qed.
+  
+End SIMMODSEM.
+
+
+
+
+(***** Move and rename: APC & HoareCall LEMMAS *****)
 
   (* Try to match bind pattern *)
-  Lemma APC_start_clo
+  Lemma APC_start_clo Σ
     I fls flt r g ps pt {R} RR st_src k_src sti_tgt  
     at_most o stb 
   :
-    @isim _ I fls flt r g R RR true pt (st_src, _APC stb at_most o >>= (fun x => tau;; Ret x) >>= k_src) sti_tgt
+    @isim Σ I fls flt r g R RR true pt (st_src, _APC stb at_most o >>= (fun x => tau;; Ret x) >>= k_src) sti_tgt
   -∗  
     @isim _ I fls flt r g R RR ps pt (st_src, interp_hEs_hAGEs stb o (trigger hAPC) >>= k_src) sti_tgt.
   Proof.
@@ -258,11 +334,11 @@ Section SIMMODSEM.
     iApply "K".
   Qed.
 
-  Lemma APC_stop_clo
+  Lemma APC_stop_clo Σ
     I fls flt r g ps pt {R} RR st_src k_src sti_tgt  
     at_most o stb
   :
-    @isim _ I fls flt r g R RR true pt (st_src, k_src tt) sti_tgt
+    @isim Σ I fls flt r g R RR true pt (st_src, k_src tt) sti_tgt
   -∗  
     @isim _ I fls flt r g R RR ps pt (st_src, _APC stb at_most o >>= (fun x => (tau;; Ret x) >>= k_src)) sti_tgt.
   Proof.
@@ -272,13 +348,13 @@ Section SIMMODSEM.
     force. instantiate (1:= true). steps. eauto.
   Qed.
   
-  Lemma APC_step_clo
+  Lemma APC_step_clo Σ
     I fls flt r g ps pt {R} RR st_src k_src sti_tgt  
     at_most o stb next fn vargs fsp
     (SPEC: stb fn = Some fsp)
     (NEXT: (next < at_most)%ord)
   :
-    @isim _ I fls flt r g R RR true pt (st_src, HoareCall true o fsp fn vargs >>= (fun _ => _APC stb next o) >>= (fun x => tau;; Ret x) >>= k_src) sti_tgt
+    @isim Σ I fls flt r g R RR true pt (st_src, HoareCall true o fsp fn vargs >>= (fun _ => _APC stb next o) >>= (fun x => tau;; Ret x) >>= k_src) sti_tgt
   -∗  
     @isim _ I fls flt r g R RR ps pt (st_src, _APC stb at_most o >>= (fun x => (tau;; Ret x) >>= k_src)) sti_tgt.
   Proof.
@@ -293,7 +369,7 @@ Section SIMMODSEM.
     Unshelve. eauto.
   Qed.
 
-  Lemma hcall_clo
+  Lemma hcall_clo Σ
     I fls flt r g ps pt {R} RR st_src st_tgt k_src k_tgt
     fn varg_src varg_tgt o X (x: shelve__ X) (D: X -> ord) P Q
     (* PURE, ... *)
@@ -304,7 +380,7 @@ Section SIMMODSEM.
       ∗ I st_src st_tgt 
       ∗ (∀st_src0 st_tgt0 vret_src vret_tgt, 
              (Q x vret_src vret_tgt ∗ I st_src0 st_tgt0) 
-          -∗ @isim _ I fls flt r g R RR true true (st_src0, k_src vret_src) (st_tgt0, k_tgt vret_tgt)))
+          -∗ @isim Σ I fls flt r g R RR true true (st_src0, k_src vret_src) (st_tgt0, k_tgt vret_tgt)))
   -∗  
     @isim _ I fls flt r g R RR ps pt (st_src, HoareCall true o (mk_fspec D P Q) fn varg_src >>= k_src) (st_tgt, trigger (Call fn varg_tgt) >>= k_tgt).
   Proof.
@@ -316,385 +392,3 @@ Section SIMMODSEM.
     call; [eauto|].
     steps. iApply "K". iFrame.
   Qed.
-
-  (****************************)
-
-  Local Notation universe := positive.
-  (* Local Notation level := nat. *)
-
-  (* Lemma initialized0_unique k : initialized0 k -∗ initialized0 k -∗ False.
-  Proof. 
-    iIntros "I0 I1". iCombine "I0 I1" as "I".
-    iOwnWf "I". clear -H2.
-    rr in H2. ur in H2. unseal "ra". des. ur in H0. ss.
-  Qed. *)
-
-  Definition init_points blk ofs f k :=  (OwnM ((blk, (ofs + k)%Z) |-> [Vint (f k)]))%I.
-  (* Definition init_points blk ofs f k := (initialized0 k ∨ OwnM ((blk, (ofs + k)%Z) |-> [Vint (f k)]))%I. *)
-
-  Fixpoint mem_index (sz: nat) : list Z :=
-      match sz with 0 => [] | S k => (Z.of_nat k) :: mem_index k end.
-
-  Definition mem_inv blk ofs f sz := ([∗ list] k ∈ (mem_index sz), init_points blk ofs f k)%I.
-
-  (* Definition initial_inv := (∀ sz, ([∗ list] k ∈ (mem_index sz), initialized0 k))%I. *)
-
-  Lemma mem_inv_split blk ofs f sz k (SZ: 0 <= k < sz): 
-    mem_inv blk ofs f sz -∗ (init_points blk ofs f k ∗ (init_points blk ofs f k -* mem_inv blk ofs f sz)).
-  Proof.
-    i. iIntros "M". iEval (unfold mem_inv) in "M". 
-    iInduction sz as [|sz0] "IH"; [lia|].
-    des. eapply lt_n_Sm_le, le_lt_eq_dec in SZ0.
-    destruct SZ0.
-    { iDestruct "M" as "[I M]".
-      iPoseProof ("IH" with "[]") as "H".
-      { iPureIntro. eauto. }
-      iPoseProof ("H" with "M") as "[I0 M]".
-      iFrame. iIntros "I". iPoseProof ("M" with "I") as "M". iFrame.
-    }
-    iClear "IH". iDestruct "M" as "[I M]". subst. iFrame. eauto.
-  Qed. 
-
-  Lemma mem_inv_set blk ofs f sz k (SZ: 0 <= k < sz):
-    mem_inv blk ofs f sz -∗ (∀x, init_points blk ofs f k ∗ (OwnM ((blk, (ofs + k)%Z) |-> [Vint x]) -∗ mem_inv blk ofs (fun n => if Z.eq_dec n k then x else (f n)) sz)).
-  Proof.
-    induction sz; [lia|].
-    destruct (classic (k = sz)); cycle 1.
-    {
-      iIntros "H %". unfold mem_inv. s.
-      iDestruct "H" as "[H0 H1]".
-      replace (init_points blk ofs (λ n : Z, if Z.eq_dec n k then x else f n) sz) with (init_points blk ofs f sz).
-      2: { unfold init_points. destruct (Z.eq_dec sz k); [lia|ss]. }
-      iPoseProof (IHsz with "H1") as "H1"; [lia|]. 
-      iSpecialize ("H1" $! x). iDestruct "H1" as "[H1 H2]".
-      iFrame. iApply "H2".
-    }
-    clear IHsz SZ. subst.
-    iIntros "H %". unfold mem_inv. s.
-    iDestruct "H" as "[H0 H1]". iFrame.
-    iIntros "OWN". iSplitL "OWN".
-    { unfold init_points. des_ifs. }
-    assert (forall (sz: nat) (NONZERO: sz > 0), sz = list_max (map (Z.to_nat) (mem_index sz)) + 1).
-    { 
-      i. induction sz0; [lia|].  
-      s. destruct (classic (sz0 = 0)).
-      { rewrite H1. eauto. }
-      { assert (sz0 > 0) by lia. specialize (IHsz0 H2).
-        replace (Z.to_nat sz0 `max` list_max (map Z.to_nat (mem_index sz0))) with (Z.to_nat sz0); lia.
-      }
-    }
-    destruct (classic (sz = 0)).
-    { rewrite H2. ss. }
-    assert (sz > 0) by lia. hexploit (H1 sz H3).
-    generalize sz at 2 3 7. i. 
-
-
-    assert (sz > list_max (map Z.to_nat (mem_index sz0))) by lia. 
-    clear H2 H3 H4.
-    iStopProof. induction sz0; eauto. s.
-    iIntros "[H0 H1]". iSplitL "H0".
-    { unfold init_points. des_ifs. simpl in H5. lia. }
-    iApply IHsz0; eauto. simpl in H5. lia.
-  Qed.
-
-  Definition init_map_st := (fun (_: Z) => 0%Z, 0%Z).
-  
-  Let Ist: Any.t -> Any.t -> iProp := 
-    (fun st_src st_tgt =>
-             ((∃ blk ofs (f: Z -> Z) (sz: Z), 
-                ⌜st_src = Any.pair (f, sz)↑ tt↑ /\  st_tgt = Any.pair (Vptr blk ofs)↑ tt↑⌝ 
-                ∗ mem_inv blk ofs f (Z.to_nat sz) ∗ pending0) 
-             ∨ (⌜st_src = Any.pair init_map_st↑ tt↑ /\ st_tgt = Any.pair Vnullptr↑ tt↑⌝))%I).
-             (* ∨ (∃ st_src0 st_tgt0, callable ∗ mapstate (st_src0, st_tgt0) ∗ ⌜st_src = st_src0↑ /\ st_tgt = st_tgt0↑⌝). *)
-
-  Let Mem := HMem (fun _ => false).
-
-  Theorem sim: HModPair.sim (HMod.add (MapM.HMap GlobalStbM) Mem) (HMod.add MapI.Map Mem) Ist.
-  Proof.  
-  Admitted.
-    (* Takes 9 minutes for Qed *)
-
-    (* sim_init.
-    - iIntros "[H0 H1]". iFrame. iRight. eauto.
-    - unfold cfunU, initF, MapI.initF, interp_sb_hp, HoareFun, ccallU. s.
-      st. (* need to optimize *)
-      iDestruct "ASM" as "(W & (%Y & %M & P0) & %X)". subst.
-      st.
-      iDestruct "IST" as "[IST|%]".
-      {
-        iDestruct "IST" as (? ? ? ?) "(_ & _ & P)".
-        iExFalso. iApply (pending0_unique with "P P0").
-      }
-      des. subst.
-      inline_r. 
-      st. force. instantiate (1:= x).
-      st. force. instantiate (1:= [Vint x]↑).
-      st. force. iSplitR. { eauto. }
-      st. rewrite interp_hAGEs_hapc. st.
-      unfold HoareAPC. st.
-      rewrite unfold_APC.
-      st. destruct y0; cycle 1.
-      { unfold guarantee, triggerNB. st. inv y6. }
-      unfold ModSem.run_l. rewrite ! Any.pair_split. fold ModSem.run_l.
-      st. iDestruct "GRT" as "[GRT %]". iDestruct "GRT" as ( ? ) "(% & POINTS)". subst. st.
-      unfold ModSem.run_l. rewrite ! Any.pair_split. fold ModSem.run_l.
-      st. force. st. force. iSplitL "W". { eauto. }
-      rewrite Any.upcast_downcast in G. inv G. inv G0. st.
-      pattern 0%Z at 36.
-      match goal with
-      | |- ?P 0%Z => cut (P (x-x)%Z)
-      end; ss.
-      { rewrite Z.sub_diag. ss. }
-      assert (OWN: OwnM ((b, 0%Z) |-> repeat Vundef x) -∗ OwnM ((b, 0%Z) |-> (repeat (Vint 0) (x - x) ++ repeat Vundef x))).
-      { iIntros "H". rewrite Nat.sub_diag. ss. }
-      iPoseProof (OWN with "POINTS") as "O".
-      iStopProof. cut (x <= x); [|lia].
-      generalize x at 1 4 5 11. intros n. induction n; i; iIntros "(P0 & O)".
-      { 
-        rewrite unfold_iter. st. destruct (Z_lt_le_dec (x - 0) x).
-        { exfalso. lia. }
-        st. iSplitL; [|eauto].
-        iLeft. iFrame. iExists b, 0%Z, (fun _ => 0%Z), x.
-        iSplit; eauto. unfold mem_inv, init_points.
-        replace (x - 0) with x; [|lia].
-        rewrite app_nil_r.
-        iStopProof. induction x; eauto.
-        iIntros "O"; s. 
-        replace (Z.to_nat (Z.pos (Pos.of_succ_nat x))) with (S x); [|lia].
-        rewrite repeat_cons. rewrite points_to_app.
-        iDestruct "O" as "[H0 H1]". rewrite repeat_length.
-        iPoseProof (IHx with "H0") as "IH"; [lia| |lia|lia| ].
-        {
-          replace (x-x) with 0; [|lia].
-          iIntros "H". rewrite points_to_app. rewrite repeat_length. s.
-          rewrite points_to_nil. r_solve. 
-          replace (0 + 0)%Z with 0%Z; [eauto|lia].
-        }
-        replace (Z.to_nat x) with x; [|lia]. iFrame.
-      }
-
-      rewrite unfold_iter. st.
-      destruct (Z_lt_le_dec (x - Z.pos (Pos.of_succ_nat n)) x).
-      2: { exfalso. lia. }
-      st. unfold scale_int at 1.
-      destruct (Zdivide_dec 8 ((x - Z.pos (Pos.of_succ_nat n)) * 8)).
-      2: { exfalso. eapply n0. eapply Z.divide_factor_r. }
-      st.
-      assert (EQ: (0 + ((x - S n)%nat * 8) `div` 8) = (x - S n)).
-      { rewrite Nat.div_mul; ss. }
-      assert (
-        OwnM ((b, 0%Z) |-> (repeat (Vint 0) (x - S n) ++ Vundef :: repeat Vundef n))
-        -∗
-        (OwnM ((b, Z.of_nat (x - S n)) |-> [Vundef]) ** (OwnM ((b, Z.of_nat (x - S n)) |-> [Vint 0]) -* OwnM ((b, 0%Z) |-> (repeat (Vint 0) (x - n) ++ repeat Vundef n))))
-      ).
-      { 
-        iIntros "H". rewrite points_to_app. rewrite points_to_split.
-        iDestruct "H" as "[H0 [H1 H2]]". iSplitL "H1".
-        {
-          replace (x - S n: Z) with (0 + strings.length (repeat (Vint 0) (x - S n)))%Z; ss.
-          rewrite repeat_length. lia.
-        }
-        iIntros "H1". rewrite points_to_app.
-        remember ((b, 0%Z) |-> repeat (Vint 0) (x - n)).
-        remember ((b, (0 + length (repeat (Vint 0) (x - n)))%Z) |-> repeat Vundef n).
-        assert (OwnM c ∗ OwnM c0 -∗ OwnM (c ⋅ c0)).
-        { iIntros "[H0 H1]". iCombine "H0 H1" as "H". eauto. }
-        subst. iApply H2.
-        iSplitL "H0 H1".
-        {
-          assert (LEN: x - S n = length (repeat (Vint 0) (x - S n))%Z).
-          { rewrite repeat_length. refl. }
-          iEval (rewrite LEN) in "H1".
-          iCombine "H0 H1" as "H". iEval (rewrite <- points_to_app) in "H".
-          replace (repeat (Vint 0) (x - S n) ++ [Vint 0]) with (repeat (Vint 0) ((x - S n) + 1)).
-          { replace (x - S n + 1) with (x - n); ss. lia. }
-          { rewrite repeat_app; ss. }
-        }
-        replace (0 + strings.length (repeat (Vint 0) (x - n)))%Z with
-        (0 + strings.length (repeat (Vint 0) (x - S n)) + 1)%Z; ss.
-        repeat rewrite repeat_length. rewrite <- Z.add_assoc. lia.
-      }
-      
-      iPoseProof (H2 with "O") as "[H0 H1]".
-
-      inline_r.
-      replace ((0 + ((x - Z.pos (Pos.of_succ_nat n)) * 8) `div` 8))%Z with (x - S n)%Z.
-      2: { rewrite Z.div_mul; lia. }
-      st. force. instantiate (1:= (b, (x - S n)%Z, Vint 0)).
-      st. force.
-      st. force. iSplitL "H0". 
-      {   
-        iSplit; eauto. replace ((x - Z.pos (Pos.of_succ_nat n))%Z) with (x - (S n))%Z; [|lia].
-        iExists Vundef. iSplit; eauto.
-        replace (Z.of_nat (Init.Nat.sub x (S n))) with (Z.sub (Z.of_nat x) (Z.of_nat (S n))); [|lia].
-        iFrame.
-      }
-      st. rewrite interp_hAGEs_hapc. st.
-      unfold HoareAPC. st.
-      rewrite unfold_APC.
-      st. destruct y3; cycle 1.
-      { unfold guarantee, triggerNB. st. inv y5. }
-      st. iDestruct "GRT" as "((O & %) & %)". subst.
-      st. replace (x - Z.pos (Pos.of_succ_nat n) + 1)%Z with (x - n)%Z; [|lia].
-      iApply IHn; [lia|iFrame].
-      replace (Z.of_nat (Init.Nat.sub x (S n))) with (Z.sub (Z.of_nat x) (Z.of_nat (S n))); [|lia].
-      iApply ("H1" with "O").
-
-    - unfold cfunU, getF, MapI.getF, interp_sb_hp, HoareFun, ccallU. s.
-      st. iDestruct "ASM" as "(W & % & %)". subst. st.
-      iDestruct "IST" as "[IST|IST]"; cycle 1.
-      { 
-        iDestruct "IST" as "%". des. subst. 
-        unfold ModSem.run_l. rewrite ! Any.pair_split. st.
-        unfold assume. st. lia.
-      }
-      iDestruct "IST" as (? ? ? ?) "(% & (M & P))". des. subst.
-      unfold ModSem.run_l. rewrite ! Any.pair_split. fold ModSem.run_l.
-      unfold assume. st. unfold scale_int. 
-      destruct (Zdivide_dec 8 (x * 8)); cycle 1.
-      { exfalso. eapply n. eapply Z.divide_factor_r. }
-      rewrite Any.upcast_downcast in G. inv G. inv G0.
-      st. 
-      replace (ofs + (y4 * 8) `div` 8)%Z with (ofs + Z.to_nat y4)%Z; cycle 1.
-      { rewrite Z_div_mult; ss. lia. }
-      iPoseProof (mem_inv_split with "M") as "[IP M]".
-      { instantiate (1:= Z.to_nat y4). lia. }
-      inline_r.
-      st. force. instantiate (1:= (blk, (ofs + Z.to_nat y4)%Z, Vint (f (Z.to_nat y4)))).
-      st. force.
-      st. force.
-      iSplitL "W". { eauto. }
-      st. force.
-      st. force. iSplitL "IP".
-      { iSplit; eauto. }
-      st. rewrite interp_hAGEs_hapc. st.
-      unfold HoareAPC. st. rewrite unfold_APC.
-      st. destruct y3; cycle 1.
-      { unfold guarantee, triggerNB. st. inv y6. }
-      st. iDestruct "GRT" as "[[GRT %] %]". subst.
-      st. iSplitL; cycle 1.
-      { iPureIntro. do 3 f_equal. lia. }
-      iLeft. iExists blk, ofs, f, sz.
-      iPoseProof ("M" with "GRT") as "M". iFrame. eauto.
-
-    - unfold cfunU, setF, MapI.setF, interp_sb_hp, HoareFun, ccallU. s.
-      st. iDestruct "ASM" as "(W & % & %)". subst.
-      rewrite Any.upcast_downcast in G. inv G. inv G0.
-      iDestruct "IST" as "[IST|IST]"; cycle 1.
-      { 
-        iDestruct "IST" as "%". des. subst. 
-        unfold ModSem.run_l. rewrite ! Any.pair_split. fold ModSem.run_l. 
-        unfold assume. st. lia.
-      }
-      iDestruct "IST" as (? ? ? ?) "(% & M & P)". des. subst.
-      unfold ModSem.run_l. rewrite ! Any.pair_split. fold ModSem.run_l.
-      st. unfold assume. st.
-      unfold ModSem.run_l. rewrite ! Any.pair_split. fold ModSem.run_l.
-      st. 
-      unfold scale_int. destruct (Zdivide_dec 8 (y5 * 8)); cycle 1.
-      { exfalso. eapply n. eapply Z.divide_factor_r. }
-      st. force. st. force. iSplitL "W".
-      { iFrame. eauto. }
-      replace (ofs + (y5 * 8) `div` 8)%Z with (ofs + Z.to_nat y5)%Z. 
-      2: { rewrite Z_div_mult; ss. lia. }
-      iPoseProof (mem_inv_set with "M") as "M".
-      { instantiate (1:= Z.to_nat y5). lia. }
-      iSpecialize ("M" $! y6). iDestruct "M" as "[IP M]".
-      inline_r.
-      st. force. instantiate (1:= (blk, (ofs + Z.to_nat y5)%Z, Vint y6)).
-      st. force.
-      st. force. iSplitL "IP".
-      { iSplit; eauto. }
-      st. rewrite interp_hAGEs_hapc. st.
-      unfold HoareAPC. st. rewrite unfold_APC.
-      st. destruct y3; cycle 1.
-      { unfold guarantee, triggerNB. st. inv y7. }
-      st. iDestruct "GRT" as "[[O %] %]". subst.
-      st. iSplit; eauto.
-      iLeft. iExists blk, ofs, (λ n : Z, if Z.eq_dec n (Z.to_nat y5) then y6 else f n), sz.
-      iPoseProof ("M" with "O") as "M". iFrame.
-      iPureIntro. esplits; eauto.
-      repeat f_equal. extensionality x. des_ifs; lia.
-
-    - unfold cfunU, set_by_userF, MapI.set_by_userF, interp_sb_hp, HoareFun, ccallU. s.
-      st. iDestruct "ASM" as "(W & % & %)". subst.
-      rewrite Any.upcast_downcast in G. inv G. inv G0.
-      st. rewrite STB_setM. st.
-      unfold HoareCall.
-      force. Unshelve. 2: { econs. eapply y1. eapply y2. eapply (y4, y). }
-      force. instantiate (1:= [Vint y4; Vint y]↑).
-      st. force. iSplitL "W". { iFrame. eauto. }
-      call; [eauto|].
-      st. iDestruct "ASM" as "(W & _ & %)". subst.
-      force. st. force. iSplitL "W". { eauto. } 
-      rewrite G0. st. iFrame. eauto.
-
-   (***************** MEMORY FUNCTIONS ******************)
-    - unfold cfunU, Mem1.alloc_spec, interp_sb_hp, HoareFun, ccallU. s.
-      st. force. instantiate (1:= y0). 
-      st. force.
-      st. force. iSplitL "ASM"; [eauto|].
-      st. rewrite interp_hAGEs_hapc. st.
-      unfold HoareAPC. st. force. instantiate (1:= y2). 
-      rewrite unfold_APC. 
-      st. force. instantiate (1:= y3). 
-      destruct y3; cycle 1.
-      { unfold guarantee, triggerNB. st. inv y5. }
-      st. force. st. force. st. force.
-      iSplitL "GRT". { iFrame. }
-      st. eauto.
-    - unfold cfunU, Mem1.free_spec, interp_sb_hp, HoareFun, ccallU. s.
-      st. force. instantiate (1:= (y1, y2)). 
-      st. force.
-      st. force. iSplitL "ASM"; [eauto|].
-      st. rewrite interp_hAGEs_hapc. st.
-      unfold HoareAPC. st. force. instantiate (1:= y3). 
-      rewrite unfold_APC. 
-      st. force. instantiate (1:= y4). 
-      destruct y4; cycle 1.
-      { unfold guarantee, triggerNB. st. inv y6. }
-      st. force. st. force. st. force.
-      iSplitL "GRT". { iFrame. }
-      st. eauto.
-    - unfold cfunU, Mem1.load_spec, interp_sb_hp, HoareFun, ccallU. s.
-      st. force. instantiate (1:= (y0, y3, y2)). 
-      st. force.
-      st. force. iSplitL "ASM"; [eauto|].
-      st. rewrite interp_hAGEs_hapc. st.
-      unfold HoareAPC. st. force. instantiate (1:= y4). 
-      rewrite unfold_APC. 
-      st. force. instantiate (1:= y5). 
-      destruct y5; cycle 1.
-      { unfold guarantee, triggerNB. st. inv y7. }
-      st. force. st. force. st. force.
-      iSplitL "GRT". { iFrame. }
-      st. eauto.
-    - unfold cfunU, Mem1.store_spec, interp_sb_hp, HoareFun, ccallU. s.
-      st. force. instantiate (1:= (y0, y3, y2)). 
-      st. force.  
-      st. force. iSplitL "ASM"; [eauto|].
-      st. rewrite interp_hAGEs_hapc. st.
-      unfold HoareAPC. st. force. instantiate (1:= y4). 
-      rewrite unfold_APC. 
-      st. force. instantiate (1:= y5). 
-      destruct y5; cycle 1.
-      { unfold guarantee, triggerNB. st. inv y7. }
-      st. force. st. force. st. force.
-      iSplitL "GRT". { iFrame. }
-      st. eauto.
-    - unfold cfunU, Mem1.cmp_spec, interp_sb_hp, HoareFun, ccallU. s.
-      st. force. instantiate (1:= (y1, y2)).
-      st. force.
-      st. force. iSplitL "ASM"; [eauto|].
-      st. rewrite interp_hAGEs_hapc. st.
-      unfold HoareAPC. st. force. instantiate (1:= y3).
-      rewrite unfold_APC. 
-      st. force. instantiate (1:= y4). 
-      destruct y4; cycle 1.
-      { unfold guarantee, triggerNB. st. inv y6. }
-      st. force. st. force. st. force.
-      iSplitL "GRT". { iFrame. }
-      st. eauto.
-  Qed.  *)
-  
-End SIMMODSEM.
