examples/map/MapMAproof.v
@@ -19,7 +19,7 @@ From ExtLib Require Import
 Require Import ProofMode STB Invariant.
 Require Import Mem1.
 
-Require Import SimModSemFacts IProofMode IRed ITactics.
+Require Import (* SimModSemFacts *) IProofMode IRed ITactics.
 
 Require Import sProp sWorld World SRF.
 From stdpp Require Import coPset gmap namespaces.
@@ -32,10 +32,6 @@ Local Open Scope nat_scope.
 
 Section SIMMODSEM.
   Context `{_M: MapRA.t}.
-  (* Context `{_W: CtxWD.t}.
-  Context `{@GRA.inG MapRA Γ}.
-  Context `{@GRA.inG MapRA0 Γ}.
-  Context `{@GRA.inG CallableRA Γ}. *)
   Context `{@GRA.inG memRA Γ}. 
 
   Section LEMMA. 
@@ -95,10 +91,10 @@ Section SIMMODSEM.
     Proof.
       unfold initial_map, map_points_to.
       iIntros "H0 H1". iCombine "H0 H1" as "H".
-      iOwnWf "H". exfalso. rr in H2. ur in H2. unseal "ra". des.
-      rr in H3. ur in H3. unseal "ra". des.
-      rr in H3. des. ur in H3. eapply equal_f with (x:=k) in H3.
-      ur in H3. des_ifs.
+      iOwnWf "H" as WF. exfalso. rr in WF. ur in WF. unseal "ra". des.
+      rr in WF0. ur in WF0. unseal "ra". des.
+      rr in WF0. des. ur in WF0. eapply equal_f with (x:=k) in WF0.
+      ur in WF0. des_ifs.
     Qed.
 
     Lemma unallocated_range sz k v
@@ -107,10 +103,10 @@ Section SIMMODSEM.
     Proof.
       unfold unallocated, map_points_to.
       iIntros "H0 H1". iCombine "H0 H1" as "H".
-      iOwnWf "H". iPureIntro. rr in H2. ur in H2. unseal "ra". des.
-      rr in H2. ur in H3. unseal "ra".
-      rr in H3. ur in H3. unseal "ra". specialize (H3 k).
-      rr in H3. ur in H3. unseal "ra". des_ifs. lia.
+      iOwnWf "H" as WF. iPureIntro. rr in WF. ur in WF. unseal "ra". des.
+      rr in WF. ur in WF0. unseal "ra".
+      rr in WF0. ur in WF0. unseal "ra". specialize (WF0 k).
+      rr in WF0. ur in WF0. unseal "ra". des_ifs. lia.
     Qed.
 
     Lemma black_map_get f k v
@@ -119,52 +115,40 @@ Section SIMMODSEM.
     Proof.
       unfold black_map, map_points_to.
       iIntros "H0 H1". iCombine "H0 H1" as "H".
-      iOwnWf "H". iPureIntro. rr in H2. ur in H2. unseal "ra". des.
-      rr in H3. ur in H3. unseal "ra". des.
-      rr in H3. des. ur in H3. eapply equal_f with (x:=k) in H3.
-      ur in H3. des_ifs.
+      iOwnWf "H" as WF. iPureIntro. rr in WF. ur in WF. unseal "ra". des.
+      rr in WF0. ur in WF0. unseal "ra". des.
+      rr in WF0. des. ur in WF0. eapply equal_f with (x:=k) in WF0.
+      ur in WF0. des_ifs.
     Qed.
 
     Lemma black_map_set f k w v
       :
-      black_map f -∗ map_points_to k w -∗ #=> (black_map (fun n => if Z.eq_dec n k then v else f n) ∗ map_points_to k v).
+      black_map f -∗ map_points_to k w -∗ #=> (black_map (<[k:=v]>f) ∗ map_points_to k v).
     Proof.
       iIntros "H0 H1". iCombine "H0 H1" as "H".
       iPoseProof (OwnM_Upd with "H") as "H".
-      { instantiate (1:=black_map_r (fun n => if Z.eq_dec n k then v else f n) ⋅ map_points_to_r k v).
-        rr. i. ur in H2. ur. unseal "ra". des_ifs. des. split; auto.
-        ur in H3. ur. des_ifs. des. rr in H3. des. split.
-        { rr. exists ctx. ur in H3. ur. extensionality n.
-          eapply equal_f with (x:=n) in H3. ur in H3. ur. des_ifs.
+      { instantiate (1:=black_map_r (<[k:=v]>f) ⋅ map_points_to_r k v).
+        rr. intros ctx WF. ur in WF. ur. unseal "ra". des_ifs. des. split; auto.
+        ur in WF0. ur. des_ifs. des. rr in WF0. des. split.
+        { rr. exists ctx. ur in WF0. ur. extensionality n.
+          eapply equal_f with (x:=n) in WF0. ur in WF0. ur.
+          des_ifs; rewrite ->?fn_lookup_insert, ?fn_lookup_insert_ne; eauto.
         }
         { ur. i. rr. ur. unseal "ra". ss. }
       }
       iMod "H". iDestruct "H" as "[H0 H1]". iFrame. auto.
     Qed.
 
-
     Lemma pending_unique:
       pending -∗ pending -∗ False%I.
     Proof.
       iIntros "H0 H1". iCombine "H0 H1" as "H".
-      iOwnWf "H". exfalso. clear - H2.
-      rr in H2. ur in H2. unseal "ra". des.
-      rr in H2. ur in H2. unseal "ra". ss.
+      iOwnWf "H" as WF. exfalso.
+      rr in WF. ur in WF. unseal "ra". des.
+      rr in WF. ur in WF. unseal "ra". ss.
     Qed.
+    
   End LEMMA.
-
-  Local Notation universe := positive.
-  (* Local Notation level := nat. *)
-
-  (* 
-    isim_apc_src : src hAPC, tgt HoareCall true(pure)
-  *)
-
-  Definition is_possibly_pure (fsp: fspec): Prop := exists x, is_pure (fsp.(measure) x).
-
-  Definition stb_pure_incl (stb_tgt stb_src: string -> option fspec): Prop :=
-    forall fn fsp (FIND: stb_tgt fn = Some fsp) (PURE: is_possibly_pure fsp), stb_src fn = Some fsp
-  .
 
   Variable GlobalStb: Sk.t -> gname -> option fspec.
   Hypothesis STB_set: forall sk, (GlobalStb sk) "set" = Some set_spec.
@@ -172,191 +156,149 @@ Section SIMMODSEM.
   Variable GlobalStbM: Sk.t -> gname -> option fspec.
   Hypothesis STB_setM: forall sk, (GlobalStbM sk) "set" = Some set_specM.
 
-  (* Hypothesis PUREINCL: forall sk, stb_pure_incl (GlobalStbM sk) (GlobalStb sk). *)
+  (* TODO: Try spawn & consume a dummy world *)
+  Definition Ist: Any.t -> Any.t -> iProp :=
+    (fun st_src st_tgt =>
+       ((pending0 ∗ initial_map ∗ ⌜st_src = (fun (_: Z) => 0%Z)↑ /\ st_tgt = (fun (_: Z) => 0%Z, 0%Z)↑⌝)
+        ∨ 
+        (pending ∗ ∃ f sz, ⌜st_src = f↑ /\ st_tgt = (f, sz)↑⌝ ∗ black_map f ∗ unallocated sz))%I).
 
-
-  From Ordinal Require Import Ordinal.
-
-  Lemma isim_apc 
-    I fls flt r g ps pt {R} RR st_src st_tgt k_src k_tgt stb_src stb_tgt
-    (* (STBINCL: stb_pure_incl stb_tgt stb_src) *)
-  :
-    (I st_src st_tgt ∗ (∀st_src0 st_tgt0 vret, (I st_src0 st_tgt0) -∗ isim I fls flt r g RR true true (st_src0, k_src vret) (st_tgt0, k_tgt vret)))
-  -∗
-    @isim _ I fls flt r g R RR ps pt (st_src, interp_hEs_hAGEs stb_src ord_top (trigger hAPC) >>= k_src) (st_tgt, interp_hEs_hAGEs stb_tgt ord_top (trigger hAPC) >>= k_tgt).
+  Lemma simF_init:
+    HModPair.sim_fun
+      (MapA.HMap GlobalStb) (MapM.HMap GlobalStbM) Ist "init".
   Proof.
-    (* iIntros "[IST K]".
-    unfold interp_hEs_hAGEs. rewrite! interp_trigger. grind.
-    unfold HoareAPC. grind.
-    choose. instantiate (1:= x).
-    induction ord_top.
-    { rewrite ! unfold_APC. steps. 
-      force. instantiate (1:= y).
-      destruct y; steps.
-      { iApply "K"; eauto. }
-    }
-
-
-    (****)
-    rewrite! unfold_APC.
-    choose. instantiate (1:= x0).
-    destruct x0 eqn: Eqx.
-    { steps. iApply "K". eauto. }
-    choose. instantiate (1:= x1).
-    unfold guarantee.
-    choose. rewrite! bind_ret_l. choose. instantiate (1:= x3).
-    destruct x3. steps. 
-    unfold HoareCall.
-    choose. instantiate (1:= x3).
-    choose. instantiate (1:= x4).
-    steps. force. iSplitL "GRT"; [eauto|].
-    prep. call; eauto.
-    take. instantiate (1:= x5).
-    steps. force. iSplitL "ASM"; [eauto|].
-    steps.  *)
-  Admitted.
-
-  Ltac apc := prep; iApply isim_apc; iSplitL "IST"; [eauto|iIntros "% % %"; iIntros "IST"].
-
-  (* Lemma isim_call_impure
-    I fls flt r g ps pt {R} RR st_src st_tgt k_src k_tgt 
-    fn args stb_src stb_tgt
-  :
-    (I st_src st_tgt ∗ (∀st_src0 st_tgt0 vret, (I st_src0 st_tgt0) -∗ isim I fls flt r g RR true true (st_src0, k_src vret) (st_tgt0, k_tgt vret)))
-  -∗
-    @isim _ I fls flt r g R RR ps pt (st_src, HoareCall false ord_top stb_src fn args >>= k_src) (st_tgt, HoareCall false ord_top stb_tgt fn args >>= k_tgt).
-  Proof.
-    iIntros "[IST K]".
-    rewrite ! HoareCall_parse. unfold HoareCallPre.
-    steps.
+    r. i. pattern (MapA.HMap GlobalStb) at 1. rewrite MapA.HMap_unfold. s.
+    pattern (MapM.HMap GlobalStbM) at 1. rewrite MapM.HMap_unfold. s. i. iIntros "IST".
     
+    unfold cfunU, initF, MapM.initF, interp_sb_hp, HoareFun. s.
+    take. instantiate (1:= x). destruct x. 
+    take. instantiate (1:= x0).
+    asm. iDestruct "ASM" as "(W & (%Y & %M & P) & %X)". subst.
+    iDestruct "IST" as "[(P0 & INIT & %)|(P' & _)]"; cycle 1.
+    { iExFalso. iApply (pending_unique with "P P'"). } 
+    iPoseProof (initial_map_initialize with "INIT") as "(BLACK & INIT & UNALLOC)". instantiate (1:= x).
+    iSplitL "P0 W".
+    { iFrame. esplits; eauto. }  
+    st. des. subst. rewrite Any.upcast_downcast in G. inv G.
+    force. instantiate (1:= y).
+    force. iDestruct "GRT" as "(CW & %Y)". des. subst. iSplitL "CW INIT". 
+    { iFrame. iSplit; eauto. }
+    st. iSplit; eauto.
+    iRight. iFrame. iExists (λ _ : Z, 0%Z), x. iFrame. eauto.
+  Qed.
+
+  Variable FFF : forall (P: Prop), P.
   
-  Admitted. *)
+  Lemma simF_get:
+    HModPair.sim_fun
+      (MapA.HMap GlobalStb) (MapM.HMap GlobalStbM) Ist "get".
+  Proof.
+    r. i. pattern (MapA.HMap GlobalStb) at 1. rewrite MapA.HMap_unfold. s.
+    pattern (MapM.HMap GlobalStbM) at 1. rewrite MapM.HMap_unfold. s. i. iIntros "IST".
 
-(* TODO: Try spawn & consume a dummy world *)
-  Let Ist: Any.t -> Any.t -> iProp :=
-        (fun st_src st_tgt =>
-             ((∃ f sz, pending ∗ ⌜st_src = f↑ /\ st_tgt = (f, sz)↑⌝ ∗ black_map f ∗ unallocated sz) ∨ 
-             (pending0 ∗ ⌜st_src = (fun (_: Z) => 0%Z)↑ /\ st_tgt = (fun (_: Z) => 0%Z, 0%Z)↑⌝ ∗ initial_map))%I).
+    unfold cfunU, getF, MapM.getF, interp_sb_hp, HoareFun. s.
+    st. iDestruct "ASM" as "(WORLD & (% & MAP) & %)". subst.
+    rewrite Any.upcast_downcast in G. inv G. inv G0.
+    iDestruct "IST" as "[(_ & INIT & _)|(P & IST)]".
+    { iExFalso. iApply (initial_map_no_points_to with "INIT MAP"). }
+    iDestruct "IST" as (? ?) "(% & BLACK & UNALLOC)".
+    force. instantiate (1:= mk_meta y0 y1 y3).
+    force. instantiate (1:= [Vint y3]↑).
+    force. iSplitL "WORLD". { iFrame. eauto. }
+    des. subst. st. 
+    iPoseProof (unallocated_range with "UNALLOC MAP") as "%".
+    iPoseProof (black_map_get with "BLACK MAP") as "%".
+    subst. force. st.
+    iDestruct "GRT" as "(WORLD & %)". des. subst.
+    force. iSplitL "WORLD MAP". { iFrame. eauto. }
+    st. iSplitL; eauto. iRight.
+    iFrame. iExists f, sz. iFrame. eauto.
 
+    Unshelve. all: eauto.
+  Qed.
+
+  Lemma simF_set:
+    HModPair.sim_fun
+      (MapA.HMap GlobalStb) (MapM.HMap GlobalStbM) Ist "set".
+  Proof.
+    r. i. pattern (MapA.HMap GlobalStb) at 1. rewrite MapA.HMap_unfold. s.
+    pattern (MapM.HMap GlobalStbM) at 1. rewrite MapM.HMap_unfold. s. i. iIntros "IST".
+
+    unfold cfunU, setF, MapM.setF, interp_sb_hp, HoareFun. s.
+    st. iDestruct "ASM" as "(WORLD & (% & MAP) & %)". subst. 
+    iDestruct "IST" as "[(_ & INIT & _)|(P & IST)]".
+    { iExFalso. iApply (initial_map_no_points_to with "INIT MAP"). }
+    iDestruct "IST" as (? ?) "(% & BLACK & UNALLOC)". 
+    force. instantiate (1:= mk_meta y0 y1 (x2, x1)).
+    force. instantiate (1:= [Vint x2; Vint x1]↑).
+    force. iSplitL "WORLD". { iFrame. eauto. }
+    des. subst. st. 
+    iPoseProof (unallocated_range with "UNALLOC MAP") as "%".
+    iPoseProof (black_map_set with "BLACK MAP") as ">(BLACK & MAP)". instantiate (1:= y5).
+    subst. force. st.
+    iDestruct "GRT" as "(WORLD & %)". des; subst.
+    rewrite Any.upcast_downcast in G. inv G. inv G0. 
+    force. iSplitL "WORLD MAP". { iFrame. eauto. } 
+    st. iSplit; eauto.
+    iRight. iFrame. iExists (<[y4:=y5]> f), sz.
+    iFrame. eauto.
+
+    Unshelve. all: eauto.
+  Qed.
+
+  Lemma simF_set_by_user:
+    HModPair.sim_fun
+      (MapA.HMap GlobalStb) (MapM.HMap GlobalStbM) Ist "set_by_user".
+  Proof.
+    r. i. pattern (MapA.HMap GlobalStb) at 1. rewrite MapA.HMap_unfold. s.
+    pattern (MapM.HMap GlobalStbM) at 1. rewrite MapM.HMap_unfold. s. i. iIntros "IST".
+
+    unfold cfunU, set_by_userF, MapM.set_by_userF, interp_sb_hp, HoareFun. s.
+    st. iDestruct "ASM" as "(WORLD & (% & MAP) & %)". subst.
+    iDestruct "IST" as "[(_ & INIT & _)|(P & IST)]".
+    { iExFalso. iApply (initial_map_no_points_to with "INIT MAP"). }
+    iDestruct "IST" as (? ?) "(% & BLACK & UNALLOC)". des. subst.
+    rewrite Any.upcast_downcast in G. inv G. inv G0.
+    force. instantiate (1:= mk_meta y0 y1 y3).
+    force. instantiate (1:= [Vint y3]↑).
+    force. iSplitL "WORLD". { iFrame. eauto. }
+    st. unfold ccallU. st. rewrite STB_set. st.
+    rewrite STB_setM in G0. inv G0.
+    apply Any.downcast_upcast in G. des. subst.
+    rewrite! HoareCall_parse. unfold HoareCallPre.
+    st. iDestruct "GRT" as "[[WORLD [% %]] _]". subst.
+    apply Any.upcast_inj in H3. des. depdes EQ0.
+    force. instantiate (1:= mk_meta y4 y5 (_, _, _)).
+    force. instantiate (1:= Any.upcast [Vint _; Vint _]).
+    st. force. iSplitL "WORLD MAP".
+    { iFrame. eauto. }
+    st. iCombine "P BLACK UNALLOC" as "IST". call.
+    { iRight. iDestruct "IST" as "(P & B & U)".
+      iFrame. iExists f, sz. iFrame. eauto.
+    }
+    unfold HoareCallPost.
+    st. iDestruct "ASM" as "(WORLD & (% & MAP) & %)". subst.
+    rewrite Any.upcast_downcast in G. depdes G.
+    force. (*TODO: what is it? *) prep. asm_r.
+    iDestruct "IST" as "[(_ & INIT & _)|(P & IST)]".
+    { iExFalso. iApply (initial_map_no_points_to with "INIT MAP"). }
+    iSplitL "WORLD". { iFrame. eauto. }
+    st. iDestruct "GRT" as "(WORLD & %)".
+    force. des. subst. iSplitL "WORLD MAP". { iFrame. eauto. }
+    st. iSplitL; eauto.
+    iRight. iFrame.    
+  Qed.
+  
   Theorem sim: HModPair.sim (MapA.HMap GlobalStb) (MapM.HMap GlobalStbM) Ist.
   Proof.
-  Admitted.
-
-  (* Proved *)
-    (* sim_init.
-    - iIntros "(IST & P & INIT0)"; s. iSplitL "INIT0"; eauto.  
-      iRight. iFrame. eauto. 
-    - unfold cfunU, initF, MapM.initF, interp_sb_hp, HoareFun. s.
-      take. instantiate (1:= x). destruct x. 
-      take. instantiate (1:= x0).
-      asm. iDestruct "ASM" as "(W & (%Y & %M & P) & %X)". subst.
-      iDestruct "IST" as "[IST|(P0 & % & INIT)]".      
-      { (* Precondition *)
-        iDestruct "IST" as (? ?) "(P' & _)".
-        iExFalso. iApply (pending_unique with "P P'"). 
-      } 
-      iPoseProof (initial_map_initialize with "INIT") as "(BLACK & INIT & UNALLOC)". instantiate (1:= x).
-      iSplitL "P0 W".
-      { iFrame. esplits; eauto. }  
-      steps. 
-      des. subst. rewrite Any.upcast_downcast in G. inv G.
-      force. instantiate (1:= y).
-      force. iSplitL "GRT INIT". 
-      { (* Postcondition *)
-        iDestruct "GRT" as "(W & _ & %Y)". iFrame.
-        iSplit; eauto. 
-      }
-      steps. iSplit; eauto.
-      iLeft. iExists (λ _ : Z, 0%Z), x. iFrame. eauto. 
-
-    - unfold cfunU, getF, MapM.getF, interp_sb_hp, HoareFun. s.
-      steps. iDestruct "ASM" as "(WORLD & (% & MAP) & %)". subst.
-      rewrite Any.upcast_downcast in G. inv G. inv G0.
-      iDestruct "IST" as "[IST|IST]"; cycle 1.
-      {
-        iExFalso. iDestruct "IST" as "(_ & _ & INIT)".
-        iApply (initial_map_no_points_to with "INIT MAP").
-      }
-      iDestruct "IST" as (? ?) "(P & % & BLACK & UNALLOC)".
-      force. instantiate (1:= mk_meta y1 y2 y4).
-      force. instantiate (1:= [Vint y4]↑).
-      force. iSplitL "WORLD". { eauto. }
-      des. subst. steps. 
-      iPoseProof (unallocated_range with "UNALLOC MAP") as "%".
-      iPoseProof (black_map_get with "BLACK MAP") as "%".      
-      subst. force. steps.
-      iDestruct "GRT" as "(WORLD & _ & %)".
-      force. iSplitL "WORLD MAP". { iFrame. eauto. }  
-      steps. iSplitL; eauto. iLeft.
-      iExists f, sz. iFrame. eauto.
-
-    - unfold cfunU, setF, MapM.setF, interp_sb_hp, HoareFun. s.
-      steps. iDestruct "ASM" as "(WORLD & (% & MAP) & %)". subst. 
-      iDestruct "IST" as "[IST|IST]"; cycle 1.
-      {
-        iExFalso. iDestruct "IST" as "(_ & _ & INIT)".
-        iApply (initial_map_no_points_to with "INIT MAP").
-      }
-      iDestruct "IST" as (? ?) "(P & % & BLACK & UNALLOC)". 
-      force. instantiate (1:= mk_meta y1 y2 (x2, x1)).
-      force. instantiate (1:= [Vint x2; Vint x1]↑).
-      force. iSplitL "WORLD". { eauto. }
-      des. subst. steps. 
-      iPoseProof (unallocated_range with "UNALLOC MAP") as "%".
-      iPoseProof (black_map_set with "BLACK MAP") as ">(BLACK & MAP)". instantiate (1:= y6).
-      subst. force. steps.
-      iDestruct "GRT" as "(WORLD & _ & %)".
-      rewrite Any.upcast_downcast in G. inv G. inv G0. 
-      force. iSplitL "WORLD MAP". { iFrame. eauto. } 
-      steps. iSplit; eauto.
-      iLeft. iExists (λ n : Z, if Z.eq_dec n y5 then y6 else f n), sz.
-      iFrame. eauto.
-
-    - unfold cfunU, set_by_userF, MapM.set_by_userF, interp_sb_hp, HoareFun. s.
-      steps. iDestruct "ASM" as "(WORLD & (% & MAP) & %)". subst.
-      iDestruct "IST" as "[IST|IST]"; cycle 1.
-      {
-        iExFalso. iDestruct "IST" as "(_ & _ & INIT)".
-        iApply (initial_map_no_points_to with "INIT MAP").
-      }
-      iDestruct "IST" as (? ?) "(P & % & BLACK & UNALLOC)".      
-      des. subst.
-      iCombine "P BLACK UNALLOC" as "IST".
-      rewrite Any.upcast_downcast in G. inv G. inv G0.
-      force. instantiate (1:= mk_meta y1 y2 y4).
-      force. instantiate (1:= [Vint y4]↑).
-      force. iSplitL "WORLD". { iFrame. eauto. }
-      steps. unfold ccallU. steps.        
-      rewrite STB_set. steps.
-      specialize (STB_setM sk). rewrite STB_setM in G0. inv G0.
-      rewrite! HoareCall_parse. unfold HoareCallPre.
-      steps. iDestruct "GRT" as "[[WORLD [% %]] _]". 
-      subst. 
-      force. instantiate (1:= mk_meta y3 y5 (y4, x1, y)).
-      force. instantiate (1:= Any.upcast [Vint y4; Vint y]). 
-      steps. force. iSplitL "WORLD MAP".
-      { iFrame. iSplit; eauto. }
-      steps. rewrite H3. call.
-      {
-        iLeft. iExists f, sz. iDestruct "IST" as "(P & B & U)".
-        iFrame. iSplit; eauto.  
-      }
-      unfold HoareCallPost.
-      steps. iDestruct "ASM" as "(WORLD & (% & MAP) & %)". subst.
-      force. instantiate (1:= Any.upcast Vundef). instantiate (1:= Any.upcast Vundef).
-      prep. asm_r. iSplitL "WORLD". 
-      { iFrame. eauto. }
-      steps. iDestruct "GRT" as "(WORLD & _ & %)".
-      force. iSplitL "WORLD MAP".
-      { iFrame. iSplit; eauto. rewrite Any.upcast_downcast in G0. inv G0. eauto. }
-      steps. iFrame. eauto. 
-      Unshelve.
-      all: eauto.
-    Qed. *)
-
-
-
+    sim_init.
+    - iIntros "(IST & P & INIT0)"; s. iSplitL "INIT0"; eauto.
+      iLeft. iFrame. eauto.
+    - iApply simF_init. eauto.
+    - iApply simF_get. eauto.
+    - iApply simF_set. eauto.
+    - iApply simF_set_by_user. eauto.
+    Qed.
 
 End SIMMODSEM.
 
